theories/Graph.v
@@ -1,0 +1,173 @@
+Require Import Dep.Syntax.
+
+Require Import Lists.List.
+From mathcomp Require Import all_ssreflect.
+From Equations Require Import Equations.
+Set Implicit Arguments.
+Unset Strict Implicit.
+Unset Printing Implicit Defensive.
+Require Import Program. 
+Require Import Lia.
+
+Fixpoint unfold_top_recs_aux (U : countType) (n : nat) (g : gType U) :=
+if n is n'.+1 then
+  if g is GRec g' then unfold_top_recs_aux n' (g'[g])
+  else g
+else g.
+
+Fixpoint mu_height (U : countType) (g : gType U) :=
+match g with
+| GRec g0 => 1 + (mu_height g0)
+| _ => 0
+end.
+
+Definition unfold_top_recs (U : countType) (g : gType U) := 
+ unfold_top_recs_aux (mu_height g) g.
+
+
+Section AGType.
+Variable (U : countType).
+Definition act_of_gType (g : gType U) :=
+match (unfold_top_recs g) with 
+| GMsg a _ _ => Some a
+| GBranch a _ => Some a
+| _ => None
+end.
+
+Definition has_prefix (g : gType U) := act_of_gType g != None.
+
+Inductive agType := AGType g of has_prefix g.
+
+Definition agType_project ag := let: AGType g _ := ag in g.
+Canonical agType_subType := [subType for agType_project]. 
+Definition agType_eqMixin := Eval hnf in [eqMixin of agType by <:].
+Canonical agType_eqType := Eval hnf in EqType agType agType_eqMixin.
+Definition agType_choiceMixin := [choiceMixin of agType by <:].
+Canonical agType_choiceType :=
+  Eval hnf in ChoiceType agType agType_choiceMixin.
+Definition agType_countMixin := [countMixin of agType by <:].
+Canonical agType_countType := Eval hnf in CountType agType agType_countMixin.
+Canonical agType_subCountType := [subCountType of agType].
+
+Lemma action_exists : forall (ag : agType), { a : action | act_of_gType (agType_project ag) = Some a }.
+Proof. Admitted.
+
+Definition action_of_ag (ag : agType) := let: exist a _ := action_exists ag in a.
+
+
+End AGType.
+Check agType.
+Definition gType_of_agType : forall (U : countType), agType U -> gType U := agType_project.
+Coercion gType_of_agType : agType >-> gType.
+Definition action_of_agType : forall (U : countType), agType U -> action := action_of_ag.
+Coercion action_of_ag : agType >-> action.
+
+
+Section Graph.
+Variable (U : countType). 
+Check foldl.
+
+Definition g_next (g : gType U) : seq (gType U) :=
+match g with 
+| GMsg _ _ g0 => [::g0]
+| GBranch _ gs => gs
+| GPar g0 g1 => [::g0;g1]
+| GRec g0 => [::unfold_top_recs g0]
+| _ => [::]
+end.
+
+Definition ag_next (ag : agType U) : seq (agType U) := 
+ pmap insub (g_next ag).
+
+Fixpoint agType_enum_aux (n : nat) (ags : seq (agType U)) (ag : agType U) : seq (agType U) :=
+if n is n'.+1 then
+  if ag \in ags then ags
+   else foldl (agType_enum_aux n') (ag::ags) (ag_next ag)
+else ags.
+
+Fixpoint gType_size (g : gType U) :=
+match g with
+ | GMsg a u g0 => 1 + (gType_size g0)
+ | GRec g0 => 1 + (gType_size g0)
+ | GBranch a gs => 1 + (sumn (map gType_size gs))
+ | GEnd => 1
+ | GPar g0 g1 => 1 + (gType_size g0) + (gType_size g1)
+ | GVar n => 1
+end. 
+
+Definition agType_enum (ag : agType U) := agType_enum_aux (gType_size ag) ([::]) ag.
+
+Section Node.
+Variable ag : agType U.
+
+Inductive node := Node ag_n of ag_n \in (agType_enum ag).
+
+Definition node_project n := let: Node ag_n _ := n in ag_n.
+Canonical node_subType := [subType for node_project]. 
+Definition node_eqMixin := Eval hnf in [eqMixin of node by <:].
+Canonical node_eqType := Eval hnf in EqType node node_eqMixin.
+Definition node_choiceMixin := [choiceMixin of node by <:].
+Canonical node_choiceType :=
+  Eval hnf in ChoiceType node node_choiceMixin.
+Definition node_countMixin := [countMixin of node by <:].
+Canonical node_countType := Eval hnf in CountType node node_countMixin.
+Canonical node_subCountType := [subCountType of node].
+
+Definition node_next (n : node) : seq node := 
+ pmap insub (ag_next (node_project n)).
+
+Lemma in_node (n : node) : (node_project n) \in (agType_enum ag).
+Proof. Admitted.
+
+(*Lemma node_inj : injective node_project. 
+Proof. Admitted.*)
+
+Definition node_enum : seq node := pmap insub (agType_enum ag).
+
+Lemma node_enum_uniq : uniq node_enum.
+Proof. Admitted.
+
+Lemma mem_node_enum n : n \in node_enum.
+Proof. Admitted.
+
+
+Definition node_finMixin := Eval hnf in UniqFinMixin node_enum_uniq mem_node_enum.
+Canonical node_finType := Eval hnf in FinType node node_finMixin.
+Canonical node_subFinType := Eval hnf in [subFinType of node].
+
+End Node.
+End Graph.
+Arguments Node {_}.
+Check node_next.
+Arguments node_next {_} {_}.
+
+Definition agType_of_node : forall (U : countType) (g : agType U), node g -> agType U := node_project.
+Coercion agType_of_node : node >-> agType.
+
+Section Order.
+Variable (U : countType). 
+
+Definition action_from (a : action) := let : Action p0 _ _ := a in p0.
+Definition action_to (a : action) := let : Action _ p1 _ := a in p1.
+Definition action_ch (a : action) := let : Action _ _ c := a in c.
+
+Variable (ag : agType U).
+
+Definition II_rel (n0 n1 : node ag) := (action_to n0 == action_to n1).
+Definition IO_rel (n0 n1 : node ag) := (action_to n0 == action_from n1).
+Definition OO_rel (n0 n1 : node ag) := (action_from n0 == action_from n1) && (action_ch n0 == action_ch n1).
+
+Definition in_dep (n0 n1 : node ag) := [exists n', connect IO_rel n0 n' && II_rel n' n1] || II_rel n0 n1.
+Definition out_dep (n0 n1 : node ag) := connect (fun n0 n1 => OO_rel n0 n1 || IO_rel n0 n1) n0 n1.
+End Order.
+Arguments in_dep {_} {_}.
+Arguments out_dep {_} {_}.
+
+Section Linear.
+Variable (U : countType).
+
+
+Definition linear (g : gType U) := 
+if insub g is Some ag then [forall n0 : node ag, forall (n1 : node ag | action_ch n0 == action_ch n1), in_dep n0 n1 && out_dep n0 n1]
+                      else true.
+
